@prefix dc: <http://purl.org/dc/elements/1.1/> .
@prefix dcterms: <http://purl.org/dc/terms/> .
@prefix rdf: <http://www.w3.org/1999/02/22-rdf-syntax-ns#> .
@prefix rdfs: <http://www.w3.org/2000/01/rdf-schema#> .
@prefix skos: <http://www.w3.org/2004/02/skos/core#> .
@prefix skosxl: <http://www.w3.org/2008/05/skos-xl#> .
@prefix vs: <http://www.w3.org/2003/06/sw-vocab-status/ns#> .
@prefix xml: <http://www.w3.org/XML/1998/namespace> .
@prefix xsd: <http://www.w3.org/2001/XMLSchema#> .

<http://purl.org/dcx/lrmi-vocabs/accessibilityFeature/> a skos:ConceptScheme ;
    dc:title "Accessibility Features"@en ;
    dcterms:description """Content features of the resource, such as accessible
            media and alternatives."""@en ;
    dcterms:license <http://creativecommons.org/licenses/by/4.0/> .

<http://purl.org/dcx/lrmi-vocabs/accessibilityFeature/alternativeText> a skos:Concept ;
    skos:prefLabel "Alternative Text"@en ;
    skos:altLabel "alternativeText"@en ;
    skosxl:preflabel <http://purl.org/dcx/lrmi-vocabs/accessibilityFeature/label-alternativeText> ;
    skos:definition """Text that is programmatically associated with non-text
            content and that serves the equivalent purpose (WCAG2)."""@en ;
    dcterms:source <http://www.a11ymetadata.org/the-specification/>,
        <http://www.imsglobal.org/accessibility/afav3p0pd/AfA3p0_DESinfoModel_v1p0pd.html#_Toc323719836> ;
    rdfs:seeAlso <http://www.idpf.org/accessibility/guidelines/content/meta/schema.org.php> ;
    vs:term_status "unstable" ;
    skos:inScheme <http://purl.org/dcx/lrmi-vocabs/accessibilityFeature/> .

<http://purl.org/dcx/lrmi-vocabs/accessibilityFeature/annotations> a skos:Concept ;
    skos:prefLabel "Annotations"@en ;
    skosxl:preflabel <http://purl.org/dcx/lrmi-vocabs/accessibilityFeature/label-annotations> ;
    skos:altLabel "annotations"@en ;
    skos:definition """The work includes annotations from the author, instructor
            and/or others."""@en ;
    dcterms:source <http://www.a11ymetadata.org/the-specification/> ;
    vs:term_status "unstable" ;
    skos:inScheme <http://purl.org/dcx/lrmi-vocabs/accessibilityFeature/> .

<http://purl.org/dcx/lrmi-vocabs/accessibilityFeature/audioDescription> a skos:Concept ;
    skos:prefLabel "Audio Description"@en ;
    skosxl:preflabel <http://purl.org/dcx/lrmi-vocabs/accessibilityFeature/label-audioDescription> ;
    skos:altLabel "audioDescription"@en ;
    skos:definition """Narration has been added to the soundtrack to describe important visual details that
            cannot be understood from the main soundtrack alone (WCAG2)."""@en ;
    dcterms:source <http://www.a11ymetadata.org/the-specification/>,
        <http://www.imsglobal.org/accessibility/afav3p0pd/AfA3p0_DESinfoModel_v1p0pd.html#_Toc323719836> ;
    rdfs:seeAlso <http://www.idpf.org/accessibility/guidelines/content/meta/schema.org.php> ;
    vs:term_status "unstable" ;
    skos:inScheme <http://purl.org/dcx/lrmi-vocabs/accessibilityFeature/> .

<http://purl.org/dcx/lrmi-vocabs/accessibilityFeature/bookMarks> a skos:Concept ;
    skos:prefLabel "Book Marks"@en ;
    skosxl:preflabel <http://purl.org/dcx/lrmi-vocabs/accessibilityFeature/label-bookMarks> ;
    skos:altLabel "bookMarks"@en ;
    skos:definition """The work includes bookmarks to facilitate navigation to key
            points."""@en ;
    dcterms:source <http://www.a11ymetadata.org/the-specification/> ;
    vs:term_status "unstable" ;
    skos:inScheme <http://purl.org/dcx/lrmi-vocabs/accessibilityFeature/> .

<http://purl.org/dcx/lrmi-vocabs/accessibilityFeature/braille> a skos:Concept ;
    skos:prefLabel "Braille"@en ;
    skosxl:preflabel <http://purl.org/dcx/lrmi-vocabs/accessibilityFeature/label-braille> ;
    skos:altLabel "braille"@en ;
    skos:definition """Indicates that the resource is formatted in an electronic
            data format for representing braille books. Braille is a tactile system of raised dots
            representing letters of the alphabet."""@en ;
    dcterms:source <http://www.a11ymetadata.org/the-specification/>,
        <http://www.imsglobal.org/accessibility/afav3p0pd/AfA3p0_DESinfoModel_v1p0pd.html#_Toc323719845> ;
    rdfs:seeAlso <http://www.idpf.org/accessibility/guidelines/content/meta/schema.org.php> ;
    vs:term_status "unstable" ;
    skos:inScheme <http://purl.org/dcx/lrmi-vocabs/accessibilityFeature/> .

<http://purl.org/dcx/lrmi-vocabs/accessibilityFeature/captions> a skos:Concept ;
    skos:prefLabel "Captions"@en ;
    skosxl:preflabel <http://purl.org/dcx/lrmi-vocabs/accessibilityFeature/label-captions> ;
    skos:altLabel "captions"@en ;
    skos:definition """Synchronized visual and/or text alternative for both speech
            and non-speech audio information needed to understand the media content
            (WCAG2)."""@en ;
    dcterms:source <http://www.a11ymetadata.org/the-specification/>,
        <http://www.imsglobal.org/accessibility/afav3p0pd/AfA3p0_DESinfoModel_v1p0pd.html#_Toc323719846> ;
    rdfs:seeAlso <http://www.idpf.org/accessibility/guidelines/content/meta/schema.org.php> ;
    vs:term_status "unstable" ;
    skos:inScheme <http://purl.org/dcx/lrmi-vocabs/accessibilityFeature/> .

<http://purl.org/dcx/lrmi-vocabs/accessibilityFeature/ChemML> a skos:Concept ;
    skos:prefLabel "Chemical Markup Language"@en ;
    skosxl:preflabel <http://purl.org/dcx/lrmi-vocabs/accessibilityFeature/label-ChemML> ;
    skos:altLabel "ChemML"@en ;
    skos:definition """Identifies that chemical information is encoded using the
            ChemML markup language. """@en ;
    dcterms:source <http://www.a11ymetadata.org/the-specification/>,
        <http://www.imsglobal.org/accessibility/afav3p0pd/AfA3p0_DESinfoModel_v1p0pd.html#_Toc323719847> ;
    rdfs:seeAlso <http://www.idpf.org/accessibility/guidelines/content/meta/schema.org.php> ;
    vs:term_status "unstable" ;
    skos:inScheme <http://purl.org/dcx/lrmi-vocabs/accessibilityFeature/> .

<http://purl.org/dcx/lrmi-vocabs/accessibilityFeature/describedMath> a skos:Concept ;
    skos:prefLabel "Described Math"@en ;
    skosxl:preflabel <http://purl.org/dcx/lrmi-vocabs/accessibilityFeature/label-describedMath> ;
    skos:altLabel "describedMath"@en ;
    skos:definition """Textual descriptions of math equations are included, whether
            in the alt attribute for image-based equations, using the alttext attribute for MathML
            equations, or by other means."""@en ;
    vs:term_status "unstable" ;
    skos:inScheme <http://purl.org/dcx/lrmi-vocabs/accessibilityFeature/> .

<http://purl.org/dcx/lrmi-vocabs/accessibilityFeature/displayTransformability> a skos:Concept ;
    skos:prefLabel "Display Transformability"@en ;
    skosxl:preflabel <http://purl.org/dcx/lrmi-vocabs/accessibilityFeature/label-displayTransformability> ;
    skos:altLabel "displayTransformability"@en ;
    skos:definition """Display properties are controllable by the user. This
            property can be set, for example, if custom CSS style sheets can be applied to the
            content to control the appearance. It can also be used to indicate that styling in
            document formats like Word and PDF can be modified."""@en ;
    dcterms:source <http://www.a11ymetadata.org/the-specification/>,
        <http://www.w3.org/wiki/WebSchemas/Accessibility#accessibilityFeature_in_detail> ;
    rdfs:seeAlso <http://www.idpf.org/accessibility/guidelines/content/meta/schema.org.php> ;
    vs:term_status "unstable" ;
    skos:inScheme <http://purl.org/dcx/lrmi-vocabs/accessibilityFeature/> .

<http://purl.org/dcx/lrmi-vocabs/accessibilityFeature/highContrastAudio> a skos:Concept ;
    skos:prefLabel "High Contrast Audio"@en ;
    skosxl:preflabel <http://purl.org/dcx/lrmi-vocabs/accessibilityFeature/label-highContrastAudio> ;
    skos:altLabel "highContrastAudio"@en ;
    skos:definition """Audio content with speech in the foreground meets the
            contrast thresholds set out in WCAG Success Criteria 1.4.7."""@en ;
    dcterms:source <http://www.a11ymetadata.org/the-specification/>,
        <http://www.w3.org/wiki/WebSchemas/Accessibility#accessibilityFeature_in_detail> ;
    rdfs:seeAlso <http://www.idpf.org/accessibility/guidelines/content/meta/schema.org.php> ;
    vs:term_status "unstable" ;
    skos:inScheme <http://purl.org/dcx/lrmi-vocabs/accessibilityFeature/> .

<http://purl.org/dcx/lrmi-vocabs/accessibilityFeature/highContrastDisplay> a skos:Concept ;
    skos:prefLabel "High Contract Display"@en ;
    skosxl:preflabel <http://purl.org/dcx/lrmi-vocabs/accessibilityFeature/label-highContrastDisplay> ;
    skos:altLabel "highContrastDisplay"@en ;
    skos:definition """Content meets the visual contrast threshold set out in WCAG
            Success Criteria 1.4.6
            (http://www.w3.org/TR/UNDERSTANDING-WCAG20/visual-audio-contrast7.html)"""@en ;
    dcterms:source <http://www.a11ymetadata.org/the-specification/> ;
    rdfs:seeAlso <http://www.idpf.org/accessibility/guidelines/content/meta/schema.org.php> ;
    vs:term_status "unstable" ;
    skos:inScheme <http://purl.org/dcx/lrmi-vocabs/accessibilityFeature/> .

<http://purl.org/dcx/lrmi-vocabs/accessibilityFeature/index> a skos:Concept ;
    skos:prefLabel "Index"@en ;
    skosxl:preflabel <http://purl.org/dcx/lrmi-vocabs/accessibilityFeature/label-index> ;
    skos:altLabel "index"@en ;
    skos:definition "@@@"@en ;
    dcterms:source <http://www.a11ymetadata.org/the-specification/> ;
    rdfs:seeAlso <http://www.idpf.org/accessibility/guidelines/content/meta/schema.org.php> ;
    vs:term_status "unstable" ;
    skos:inScheme <http://purl.org/dcx/lrmi-vocabs/accessibilityFeature/> .

<http://purl.org/dcx/lrmi-vocabs/accessibilityFeature/largePrint> a skos:Concept ;
    skos:prefLabel "Large Print"@en ;
    skosxl:preflabel <http://purl.org/dcx/lrmi-vocabs/accessibilityFeature/label-largePrint> ;
    skos:altLabel "largePrint"@en ;
    skos:definition """The content has been formatted to meet large print
            guidelines."""@en ;
    dcterms:source <http://www.a11ymetadata.org/the-specification/> ;
    skos:note """The concept is not set if the font size can be
            increased."""@en ;
    rdfs:seeAlso <http://www.idpf.org/accessibility/guidelines/content/meta/schema.org.php> ;
    vs:term_status "unstable" ;
    skos:inScheme <http://purl.org/dcx/lrmi-vocabs/accessibilityFeature/> .

<http://purl.org/dcx/lrmi-vocabs/accessibilityFeature/latex> a skos:Concept ;
    skos:prefLabel "Latex"@en ;
    skosxl:preflabel <http://purl.org/dcx/lrmi-vocabs/accessibilityFeature/label-latex> ;
    skos:definition """Indicates that the resource is formatted to be machine
            processable by a LaTeX processor."""@en ;
    dcterms:source <http://www.a11ymetadata.org/the-specification/> ;
    rdfs:seeAlso <http://www.idpf.org/accessibility/guidelines/content/meta/schema.org.php> ;
    skos:altLabel "latex"@en ;
    vs:term_status "unstable" ;
    skos:inScheme <http://purl.org/dcx/lrmi-vocabs/accessibilityFeature/> .

<http://purl.org/dcx/lrmi-vocabs/accessibilityFeature/longDescription> a skos:Concept ;
    skos:prefLabel "Long Description"@en ;
    skosxl:preflabel <http://purl.org/dcx/lrmi-vocabs/accessibilityFeature/label-longDescription> ;
    skos:altLabel "longDescription"@en ;
    skos:definition """An alternative text that is longer than a few
            sentences."""@en ;
    dcterms:source <http://www.a11ymetadata.org/the-specification/> ;
    rdfs:seeAlso <http://www.idpf.org/accessibility/guidelines/content/meta/schema.org.php> ;
    vs:term_status "unstable" ;
    skos:inScheme <http://purl.org/dcx/lrmi-vocabs/accessibilityFeature/> .

<http://purl.org/dcx/lrmi-vocabs/accessibilityFeature/MathML> a skos:Concept ;
    skos:prefLabel "Math ML"@en ;
    skosxl:preflabel <http://purl.org/dcx/lrmi-vocabs/accessibilityFeature/label-MathML> ;
    skos:altLabel "MathML"@en ;
    skos:definition """Indicates that the resource is formatted using MathML, an
            XML-based specification for describing mathematical expressions so that they can be
            displayed, manipulated and shared over the World Wide Web
            (http://www.w3.org/Math/)."""@en ;
    dcterms:source <http://www.a11ymetadata.org/the-specification/> ;
    rdfs:seeAlso <http://www.idpf.org/accessibility/guidelines/content/meta/schema.org.php> ;
    vs:term_status "unstable" ;
    skos:inScheme <http://purl.org/dcx/lrmi-vocabs/accessibilityFeature/> .

<http://purl.org/dcx/lrmi-vocabs/accessibilityFeature/none> a skos:Concept ;
    skos:prefLabel "None"@en ;
    skosxl:preflabel <http://purl.org/dcx/lrmi-vocabs/accessibilityFeature/label-none> ;
    skos:altLabel "none"@en ;
    skos:definition "@@@"@en ;
    dcterms:source <http://www.a11ymetadata.org/the-specification/> ;
    rdfs:seeAlso <http://www.idpf.org/accessibility/guidelines/content/meta/schema.org.php> ;
    vs:term_status "unstable" ;
    skos:inScheme <http://purl.org/dcx/lrmi-vocabs/accessibilityFeature/> .

<http://purl.org/dcx/lrmi-vocabs/accessibilityFeature/printPageNumbers> a skos:Concept ;
    skos:prefLabel "Print Page Number"@en ;
    skosxl:preflabel <http://purl.org/dcx/lrmi-vocabs/accessibilityFeature/label-printPageNumbers> ;
    skos:altLabel "printPageNumber"@en ;
    skos:definition "@@@"@en ;
    dcterms:source <http://www.a11ymetadata.org/the-specification/> ;
    rdfs:seeAlso <http://www.idpf.org/accessibility/guidelines/content/meta/schema.org.php> ;
    vs:term_status "unstable" ;
    skos:inScheme <http://purl.org/dcx/lrmi-vocabs/accessibilityFeature/> .

<http://purl.org/dcx/lrmi-vocabs/accessibilityFeature/readingOrder> a skos:Concept ;
    skos:prefLabel "Reading Order"@en ;
    skosxl:preflabel <http://purl.org/dcx/lrmi-vocabs/accessibilityFeature/label-readingOrder> ;
    skos:altLabel "readingOrder"@en ;
    skos:definition "@@@"@en ;
    dcterms:source <http://www.a11ymetadata.org/the-specification/> ;
    rdfs:seeAlso <http://www.idpf.org/accessibility/guidelines/content/meta/schema.org.php> ;
    vs:term_status "unstable" ;
    skos:inScheme <http://purl.org/dcx/lrmi-vocabs/accessibilityFeature/> .

<http://purl.org/dcx/lrmi-vocabs/accessibilityFeature/signLanguage> a skos:Concept ;
    skos:prefLabel "Sign Language"@en ;
    skosxl:preflabel <http://purl.org/dcx/lrmi-vocabs/accessibilityFeature/label-signLanguage> ;
    skos:altLabel "signLanguage"@en ;
    skos:definition """A language using combinations of movements of the hands and arms, facial expressions, or body positions to convey meaning (WCAG2):
            http://www.w3.org/TR/WCAG20/#sign-languagedef."""@en ;
    dcterms:source <http://www.a11ymetadata.org/the-specification/> ;
    rdfs:seeAlso <http://www.idpf.org/accessibility/guidelines/content/meta/schema.org.php> ;
    vs:term_status "unstable" ;
    skos:inScheme <http://purl.org/dcx/lrmi-vocabs/accessibilityFeature/> .

<http://purl.org/dcx/lrmi-vocabs/accessibilityFeature/structuralNavigation> a skos:Concept ;
    skos:prefLabel "Structural Navigation"@en ;
    skosxl:preflabel <http://purl.org/dcx/lrmi-vocabs/accessibilityFeature/label-structuralNavigation> ;
        skos:altLabel "structuralNavigation"@en ;
    skos:definition "@@@"@en ;
    dcterms:source <http://www.a11ymetadata.org/the-specification/> ;
    rdfs:seeAlso <http://www.idpf.org/accessibility/guidelines/content/meta/schema.org.php> ;
    vs:term_status "unstable" ;
    skos:inScheme <http://purl.org/dcx/lrmi-vocabs/accessibilityFeature/> .

<http://purl.org/dcx/lrmi-vocabs/accessibilityFeature/tableOfContents> a skos:Concept ;
    skos:prefLabel "Table of Contents"@en ;
    skosxl:preflabel <http://purl.org/dcx/lrmi-vocabs/accessibilityFeature/label-tableOfContents> ;
    skos:altLabel "tableOfContents"@en ;
    skos:definition "@@@"@en ;
    dcterms:source <http://www.a11ymetadata.org/the-specification/> ;
    rdfs:seeAlso <http://www.idpf.org/accessibility/guidelines/content/meta/schema.org.php> ;
    vs:term_status "unstable" ;
    skos:inScheme <http://purl.org/dcx/lrmi-vocabs/accessibilityFeature/> .

<http://purl.org/dcx/lrmi-vocabs/accessibilityFeature/tactileGraphic> a skos:Concept ;
    skos:prefLabel "Tactile Graphic"@en ;
    skosxl:preflabel <http://purl.org/dcx/lrmi-vocabs/accessibilityFeature/label-tactileGraphic> ;
    skos:altLabel "tactileGraphic"@en ;
    skos:definition "@@@"@en ;
    dcterms:source <http://www.a11ymetadata.org/the-specification/> ;
    rdfs:seeAlso <http://www.idpf.org/accessibility/guidelines/content/meta/schema.org.php> ;
    vs:term_status "unstable" ;
    skos:inScheme <http://purl.org/dcx/lrmi-vocabs/accessibilityFeature/> .

<http://purl.org/dcx/lrmi-vocabs/accessibilityFeature/tactileObject> a skos:Concept ;
    skos:prefLabel "Tactile Object"@en ;
    skosxl:preflabel <http://purl.org/dcx/lrmi-vocabs/accessibilityFeature/label-tactileObject> ;
    skos:altLabel "tactileObject"@en ;
    skos:definition """@@@"""@en ;
    dcterms:source <http://www.a11ymetadata.org/the-specification/> ;
    rdfs:seeAlso <http://www.idpf.org/accessibility/guidelines/content/meta/schema.org.php> ;
    vs:term_status "unstable" ;
    skos:inScheme <http://purl.org/dcx/lrmi-vocabs/accessibilityFeature/> .

<http://purl.org/dcx/lrmi-vocabs/accessibilityFeature/taggedPDF> a skos:Concept ;
    skos:prefLabel "Tagged PDF"@en ;
    skosxl:preflabel <http://purl.org/dcx/lrmi-vocabs/accessibilityFeature/label-taggedPDF> ;
    skos:altLabel "taggedPDF"@en ;
    skos:definition "@@@"@en ;
    dcterms:source <http://www.a11ymetadata.org/the-specification/> ;
    rdfs:seeAlso <http://www.idpf.org/accessibility/guidelines/content/meta/schema.org.php> ;
    vs:term_status "unstable" ;
    skos:inScheme <http://purl.org/dcx/lrmi-vocabs/accessibilityFeature/> .

<http://purl.org/dcx/lrmi-vocabs/accessibilityFeature/timingControl> a skos:Concept ;
    skos:prefLabel "Timing Control"@en ;
    skosxl:preflabel <http://purl.org/dcx/lrmi-vocabs/accessibilityFeature/label-timingControl> ;
    skos:altLabel "timingControl"@en ;
    skos:definition "@@@"@en ;
    dcterms:source <http://www.a11ymetadata.org/the-specification/> ;
    rdfs:seeAlso <http://www.idpf.org/accessibility/guidelines/content/meta/schema.org.php> ;
    vs:term_status "unstable" ;
    skos:inScheme <http://purl.org/dcx/lrmi-vocabs/accessibilityFeature/> .

<http://purl.org/dcx/lrmi-vocabs/accessibilityFeature/transcript> a skos:Concept ;
    skos:prefLabel "Transcript"@en ;
    skosxl:preflabel <http://purl.org/dcx/lrmi-vocabs/accessibilityFeature/label-transcript> ;
    skos:altLabel "transcript"@en ;
    skos:definition "A written, typewritten, or printed copy; something transcribed or made by transcribing: http://dictionary.reference.com/browse/transcript."@en ;
    dcterms:source <http://www.a11ymetadata.org/the-specification/> ;
    rdfs:seeAlso <http://www.idpf.org/accessibility/guidelines/content/meta/schema.org.php> ;
    vs:term_status "unstable" ;
    skos:inScheme <http://purl.org/dcx/lrmi-vocabs/accessibilityFeature/> .

<http://purl.org/dcx/lrmi-vocabs/accessibilityFeature/ttsMarkup> a skos:Concept ;
    skos:prefLabel "TTS Markup"@en ;
    skosxl:preflabel <http://purl.org/dcx/lrmi-vocabs/accessibilityFeature/label-ttsMarkup> ;
    skos:altLabel "ttsMarkup"@en ;
    skos:definition "@@@"@en ;
    dcterms:source <http://www.a11ymetadata.org/the-specification/> ;
    rdfs:seeAlso <http://www.idpf.org/accessibility/guidelines/content/meta/schema.org.php> ;
    vs:term_status "unstable" ;
    skos:inScheme <http://purl.org/dcx/lrmi-vocabs/accessibilityFeature/> .

<http://purl.org/dcx/lrmi-vocabs/accessibilityFeature/unlocked> a skos:Concept ;
    skos:prefLabel "Unlocked"@en ;
    skosxl:preflabel <http://purl.org/dcx/lrmi-vocabs/accessibilityFeature/label-unlocked> ;
    skos:altLabel "unlocked"@en ;
    skos:definition "@@@"@en ;
    dcterms:source <http://www.a11ymetadata.org/the-specification/> ;
    rdfs:seeAlso <http://www.idpf.org/accessibility/guidelines/content/meta/schema.org.php> ;
    vs:term_status "unstable" ;
    skos:inScheme <http://purl.org/dcx/lrmi-vocabs/accessibilityFeature/> .

#=====================
# EXTENDED LABELS
#=====================

<http://purl.org/dcx/lrmi-vocabs/accessibilityFeature/label-alternativeText> a skosxl:label ;
    skosxl:literalForm "Alternative Text"@en .

<http://purl.org/dcx/lrmi-vocabs/accessibilityFeature/label-annotations> a skosxl:label ;
    skosxl:literalForm "Annotations"@en .

<http://purl.org/dcx/lrmi-vocabs/accessibilityFeature/label-bookMarks> a skosxl:label ;
    skosxl:literalForm "Book Marks"@en .

<http://purl.org/dcx/lrmi-vocabs/accessibilityFeature/label-braille> a skosxl:label ;
    skosxl:literalForm "Braille"@en .

<http://purl.org/dcx/lrmi-vocabs/accessibilityFeature/label-captions> a skosxl:label ;
    skosxl:literalForm "Captions"@en .

<http://purl.org/dcx/lrmi-vocabs/accessibilityFeature/label-ChemML> a skosxl:label ;
    skosxl:literalForm "Chemical Markup Language"@en .

<http://purl.org/dcx/lrmi-vocabs/accessibilityFeature/label-describedMath> a skosxl:label ;
    skosxl:literalForm "Described Math"@en .

<http://purl.org/dcx/lrmi-vocabs/accessibilityFeature/label-displayTransformability> a skosxl:label ;
    skosxl:literalForm "Display Transformability"@en .

<http://purl.org/dcx/lrmi-vocabs/accessibilityFeature/label-highContrastAudio> a skosxl:label ;
    skosxl:literalForm "High Contrast Audio"@en .

<http://purl.org/dcx/lrmi-vocabs/accessibilityFeature/label-highContrastDisplay> a skosxl:label ;
    skosxl:literalForm "High Contrast Display"@en .

<http://purl.org/dcx/lrmi-vocabs/accessibilityFeature/label-index> a skosxl:label ;
    skosxl:literalForm "Index"@en .

<http://purl.org/dcx/lrmi-vocabs/accessibilityFeature/label-largePrint> a skosxl:label ;
    skosxl:literalForm "Large Print"@en .

<http://purl.org/dcx/lrmi-vocabs/accessibilityFeature/label-latex> a skosxl:label ;
    skosxl:literalForm "Latex"@en .

<http://purl.org/dcx/lrmi-vocabs/accessibilityFeature/label-longDescription> a skosxl:label ;
    skosxl:literalForm "Long Description"@en .

<http://purl.org/dcx/lrmi-vocabs/accessibilityFeature/label-MathML> a skosxl:label ;
    skosxl:literalForm "Math ML"@en .

<http://purl.org/dcx/lrmi-vocabs/accessibilityFeature/label-none> a skosxl:label ;
    skosxl:literalForm "None"@en .

<http://purl.org/dcx/lrmi-vocabs/accessibilityFeature/label-printPageNumbers> a skosxl:label ;
    skosxl:literalForm "Print Page Number"@en .

<http://purl.org/dcx/lrmi-vocabs/accessibilityFeature/label-readingOrder> a skosxl:label ;
    skosxl:literalForm "Reading Order"@en .

<http://purl.org/dcx/lrmi-vocabs/accessibilityFeature/label-signLanguage> a skosxl:label ;
    skosxl:literalForm "Sign Language"@en .

<http://purl.org/dcx/lrmi-vocabs/accessibilityFeature/label-structuralNavigation> a skosxl:label ;
    skosxl:literalForm "Structural Navigation"@en .

<http://purl.org/dcx/lrmi-vocabs/accessibilityFeature/label-tableOfContents> a skosxl:label ;
    skosxl:literalForm "Table of Contents"@en .

<http://purl.org/dcx/lrmi-vocabs/accessibilityFeature/label-tactileGraphic> a skosxl:label ;
    skosxl:literalForm "Tactile Graphic"@en .

<http://purl.org/dcx/lrmi-vocabs/accessibilityFeature/label-taggedPDF> a skosxl:label ;
    skosxl:literalForm "Tagged PDF"@en .

<http://purl.org/dcx/lrmi-vocabs/accessibilityFeature/label-timingControl> a skosxl:label ;
    skosxl:literalForm "Timing Control"@en .

<http://purl.org/dcx/lrmi-vocabs/accessibilityFeature/label-transcript> a skosxl:label ;
    skosxl:literalForm "Transcript"@en .

<http://purl.org/dcx/lrmi-vocabs/accessibilityFeature/label-ttsMarkup> a skosxl:label ;
    skosxl:literalForm "TTS Markup"@en .

<http://purl.org/dcx/lrmi-vocabs/accessibilityFeature/label-unlocked> a skosxl:label ;
    skosxl:literalForm "Unlocked"@en .
