@prefix dc: <http://purl.org/dc/elements/1.1/> .
@prefix dcterms: <http://purl.org/dc/terms/> .
@prefix rdf: <http://www.w3.org/1999/02/22-rdf-syntax-ns#> .
@prefix rdfs: <http://www.w3.org/2000/01/rdf-schema#> .
@prefix skos: <http://www.w3.org/2004/02/skos/core#> .
@prefix skosxl: <http://www.w3.org/2008/05/skos-xl#> .
@prefix edUse: <http://purl.org/dcx/lrmi-vocabs/edUse/> .
@prefix xml: <http://www.w3.org/XML/1998/namespace> .
@prefix xsd: <http://www.w3.org/2001/XMLSchema#> .
@prefix vs: <http://www.w3.org/2003/06/sw-vocab-status/ns#> .
@prefix adms: <http://www.w3.org/ns/adms#> .
@prefix bibo: <http://purl.org/ontology/bibo/status/> .

edUse: a skos:ConceptScheme ;
    dc:title "LRMI Educational Use vocabulary" ;
    dc:creator "LRMI Task Group (DCMI)"@en-US ;
    dc:description "A concept scheme that enumerates the educational uses of a learning resource."@en-US ;
    dcterms:dateSubmitted "2015-01-21"^^xsd:date ;
    dcterms:license <http://creativecommons.org/licenses/by/4.0/> ;
    adms:status bibo:draft .
    
edUse:assessment a skos:Concept ;
    skos:prefLabel "assessment"@en-US ;
    skosxl:prefLabel edUse:label-assessment ;
    skos:definition "Primary purpose of the resource is to evaluate learning, before, during, or after instruction occurs."@en-US ;
    skos:inScheme edUse: ;
    dcterms:source "Based on Common Education Data Standards (CEDS): https://ceds.ed.gov/element/001002#Assessment"@en-US ;
    vs:term_status "unstable" .           

edUse:instruction a skos:Concept ;
    skos:prefLabel "instruction"@en-US ;
    skosxl:prefLabel edUse:label-instruction ;
    skos:definition "Primary purpose of the resource is to support the instructional process, student learning, or to provide information about the curriculum."@en-US ;
    skos:inScheme edUse: ;
    dcterms:source "Based on Common Education Data Standards (CEDS): https://ceds.ed.gov/element/001002#CurriculumInstruction"@en-US ;
    vs:term_status "unstable" .  

edUse:professionalDevelopment a skos:Concept ;
    skos:prefLabel "professional development"@en-US ;
    skosxl:prefLabel edUse:label-professionalDevelopment ;
    skos:definition "Primary purpose of the resource is to provide instruction for a teacher or other education professional."@en-US ;
    skos:inScheme edUse: ;
    dcterms:source "Based on Common Education Data Standards (CEDS): https://ceds.ed.gov/element/001002#ProfessionalDevelopment"@en-US ;  
    vs:term_status "unstable" .
    
#============================= 
# EXTENDED LABELS
#============================= 

edUse:label-instruction a skosxl:label ;
    skosxl:literalForm "instruction"@en-US .
        
edUse:label-assessment a skosxl:label ;
    skosxl:literalForm "assessment"@en-US .
    
edUse:label-professionalDevelopment a skosxl:label ;
    skosxl:literalForm "professional development"@en-US .
